\chapter{Abstract groups}
\label{ch:absgroup}

\section{Brief overview of the chapter}

\section{Groups}
\label{sec:Gsetforabstract}

We use \cref{lem:BGbytorsor} as our inspiration for trying to construct a group from an abstract group.
That is, in total analogy, we define the torsors for an abstract group,
and it will then be a relative simple matter to show that the processes of
\begin{enumerate}
\item forming the abstract group of a group and
\item taking the group represented by the torsors of an abstract group
\end{enumerate}
 are inverse to each other.
\marginnote{%
Note that we have not considered an ``abstract'' counterpart of the concept of $\infty$-group, so all we do in this section is set-based.
}
\begin{definition}
\label{def:abstrGtorsors}
If ${\agp G}=(S,e,\mu,\iota)$ is an abstract group, a \emph{$\agp G$-set}%
\index{Gset@$\agp G$-set (of abstract group)}
is a set $\mathcal X$ together with a homomorphism
$\agp G\to\abstr(\Sigma_{\mathcal X})$
from $\agp G$ to the (abstract) permutation group of $\mathcal X$:
$$Set_{\agp G}^\abstr\defequi \sum_{\mathcal X:\Set}\Hom_\abstr({\agp G},\abstr(\Sigma_{\mathcal X})).$$

The \emph{principal ${\agp G}$-torsor} $\princ {\agp G}^\abstr$ is the ${\agp G}$-set consisting of the underlying set $S$ together with the homomorphism ${\agp G}\to\abstr(\Sigma_{S})$ with underlying function of sets $S\mapsto (S=S)$ given by sending $g:S$ to $\mathrm{ua}(s\mapsto s\cdot g^{-1})$.

The type of \emph{${\agp G}$-torsors} is
$$\typetorsor_{\agp G}^\abstr\defequi\sum_{S:\Set_{\agp G}^\abstr}\Trunc{\princ {\agp G}^\abstr=S}.$$
\end{definition}
\begin{example}
  If $G$ is a group we can unravel the definition and see that an $\abstr(G)$-set consists of
  \begin{enumerate}
  \item a set $S$,
  \item a function $f:\USymG\to (S=S)$
  \item such that $f(e_G)=\refl{S}$ and for all $p,q:\USymG$ we have that $f(p\, q)=f(p)\,f(q)$.
  \end{enumerate}

\end{example}


To help reading the coming proofs we introduce some notation that is redundant, but may aid the memory in cluttered situations:  Let $x,y,z$ be elements in some type, then
\marginnote{We recognize $\preinv$ from \cref{lem:pathsptransportiseq} as the induced map of identity types $\pathsp{}\colon (y=z)\to(\pathsp y=\pathsp z)$ evaluated at $x$, while post-composition $\post$ is transport in the family $\pathsp x$.}
\begin{align*}
%  \pre:(x=y)\to ((y=z)=(x=z)),\qquad&\pre(q)(p)\defequi pq\\
  \preinv:(y=x)\to ((y=z)=(x=z)),\quad&\preinv(q)(p)\defequi\pathsp qp\defequi pq^{-1}\\
  \post:(y=z)\to ((x=y)=(x=z)),\quad&\post(p)(q)\defequi\post_pq\defequi pq\\
  %\adjoint:(x=y)\to((x=x)=(y=y)),\qquad&\adjoint(q)(p)\defequi\adjoint_qp\defequi qpq^{-1}
\end{align*}


\begin{example}\label{ex:qG}
  If $G$ is a group, then for any $x:\BG$ the principal $G$-torsor \emph{evaluated at $x$}, \ie the set $\princ Gx\defequi(\shape_G=x)$, has a natural structure of an $\abstr(G)$-set by means of
  $$\preinv:\USymG\to ((\shape_G=x)=(\shape_G=x))$$ and the fact that $\preinv(e_G)\defequi\refl{\shape_G=x}$ and that for $p,q:\USymG$ we have that
  \marginnote{\ie if $r\colon \shape_G=x$ we have that
$\preinv(p\, q)(r)=r(p\,q)^{-1}=r\,q^{-1}p^{-1}=\preinv(p)\preinv(q)(r)$  -- demonstrating why we chose $\preinv$: without the inverse this would have gone badly wrong.}
  $$\preinv(p\,q)=\preinv(p)\preinv(q).$$


That this $\abstr(G)$-set is an $\abstr(G)$-torsor then follows since $\BG$ is connected (any $\shape_G=x$ will serve as a proof of $(\shape_G=x,\preinv,!)=\princ{\abstr(G)}^\abstr$).

Though it sounded like we made a choice ending up with $\preinv$; we really didn't -- it is precisely what happens when you abstract the homomorphism $G\to\Sigma_{\princ G(x)}$:
you get the function of identity types
$$\USymG\to (\princ G(x)=\princ G(x))$$
which by the very definition of transport for $\princ G$ is $\preinv$.
\end{example}

\begin{definition}
  If ${\agp G}$ is an abstract group, then the \emph{concrete group $\concr({\agp G})$ associated with ${\agp G}$} is the group given by the pointed connected groupoid $(\typetorsor_{\agp G}^\abstr,\princ {\agp G})$.
\end{definition}
We give the construction of \cref{ex:qG} a short name since it will occur in important places.
\begin{definition}
  Let $G$ be a group.
  The group homomorphism
  $$q_G:\Hom(G,\concr(\abstr(G)))$$
  is defined in terms of the pointed map by the same name
$$q_G:\BG\to_* (\typetorsor^\abstr_{\abstr(G)},\princ {\abstr(G)}),\quad q_G(z)=(\princ G(z),\preinv,!).$$
\end{definition}

\begin{lemma}
  \label{lem:Groupsareidentitytypes}
For all groups $G$, the pointed function $q_G:G\to_*\concr(\abstr(G))$
is a  equivalence.
\end{lemma}
\begin{proof}
  To prove that $q_G$ is an equivalence it is, by \cref{cor:fib-vs-path}\ref{conn-fib-vs-path}, enough to show that if $x,y:\BG$ then the induced map
$$q_G:(x=_{\BG}y)\to (q_G(x)=q_G(y))
$$
is an equivalence.
  Now, $q_G(x)=q_G(y)$ is equivalent to the set
$$
((\shape_G=x),\preinv)=_{\abstr(G)\text{-set}}((\shape_G=y),\preinv)$$
which in turn is equivalent to
$$\sum_{f:(\shape_G=x)=(\shape_G=y)}f\preinv=\preinv f
$$
 ($f\preinv=\preinv f$ is shorthand for $\prod_{q:\shape_G=x}\prod_{p:\shape_G=p}f(pq^{-1})=f(p)q^{-1}$ and the rest of the data is redundant at the level of symmetries) and under these identities $q_G$ is given by
$$(\post,!):(x=y)\to \sum_{f:(\shape_G=x)=(\shape_G=y)}f\preinv=\preinv f.$$
Given an element
$(f,!):\sum_{f:(\shape_G=x)=(\shape_G=y)}f\preinv=\preinv f$, the preimage
$(\post,!)^{-1}(f,!)$ is equivalent to the set
$\sum_{r:x=y}(f=\post_r)$.  But if $(r,!),(s,!): \sum_{r:x=y}(f=\post_r)$, then for all $p:\shape_G=x$ we get that $r\,p=f(p)=s\,p$, that is $r=s$, so that the preimage is in fact a proposition.
To show that the preimage is contractible, it is enough to construct a function $(\shape_G=x)\to \sum_{r:x=y}(f=\post_r)$, and sending $p$ to $f(p)p^{-1}$ will do.
\end{proof}

\begin{example}
  \label{ex:abstrconcrG}
  Let ${\agp G}=(S,e,\mu,\iota)$ be an abstract group.
Then the underlying set of $\abstr(\concr({\agp G}))$ is $\princ {\agp G}^\abstr=_{\typetorsor^\abstr_{\agp G}}\princ {\agp G}^\abstr$.
Unraveling the definitions we see that this set is equivalent to
$$\sum_{p:S=S}\prod_{q,s:S}(p(s\,q^{-1})=p(s)\,q^{-1}).
$$
Setting $s\defequi e$ and renaming $t\defequi q^{-1}$ in the last equation, we see that $p(t)=p(e)t$; that is $p$ is simply multiplication with an element $p(e):S$.  in other words, the function
$$r_{\agp G}:S\to  \sum_{p:S=S}\prod_{q,s:S}(p(s\,q^{-1})=p(s)\,q^{-1}),\qquad r_{\agp G}(u)\defequi(u\cdot\,,!)
$$
is an equivalence of sets, which we by univalence is converted into an identity.
The abstract group structure of $\abstr(\concr({\agp G}))$ is given by it being the symmetries of $\princ {\agp G}^\abstr$; translated to $\sum_{p:S=S}\prod_{q,s:S}(p(s\,q^{-1})=p(s)\,q^{-1})$ this corresponds via the first projection to the symmetries of $S$.
This means that we need to know that if $u,v:S$ and consider the two symmetries $u\cdot,v\cdot:S=S$, then their composite (the operation on the symmetry on $S$) is equal to $(u\cdot v)\cdot:S=S$ (the abstract group operation), but this is true by associativity ($u\cdot(v\cdot s)=(u\cdot v)\cdot s$).  That $r_{\agp G}$ also sends $e:S$ to $\refl S$ is clear.
Hence our identity $r_{\agp G}$ underlies an identity of abstract groups
$$r_{\agp G}:{\agp G}=_{\typegroup^\abstr}\abstr(\concr({\agp G})).$$
\end{example}

This shows that every abstract group encodes the symmetries of something essentially unique.  Summing up the information we get
\begin{theorem}
  \label{thm:Groupsareidentitytypes}
  Let ${\agp G}$ be an abstract group. Then
$$\abstr:\typegroup\to\typegroup^\abstr$$ is an equivalence.
\end{theorem}

\section{Homomorphisms}
\label{sec:homabsisconcr}

Now that we know that the type of groups is identical to the type of abstract groups, it is natural to ask if the notion of group homomorphisms also coincide.

They do, and we provide two independent and somewhat different arguments.  Translating from group homomorphisms to abstract group homomorphisms is easy: if $G$ and $H$ are groups, then we defined
$$\abstr:\Hom(G,H)\to\Hom^\abstr(\abstr(G),\abstr(H))$$
in \cref{def:abstrisfunctor} as the function which takes a homomorphism, aka a pointed map $f=(\Bf_\div,p_f):\BG\ptdto\BH$ to the induced map of identity types
$$\US f\defequi \mathrm{ad}_{p_f}\ap{\Bf_\div}:\USymG\to\USymH$$
 together with the proofs that this is an abstract group homomorphism from $\abstr(G)$ to $\abstr(H)$, c.f~\cref{def:abstrisfunctor}.


Going back is somewhat more involved, and it is here we consider two approaches.
The first is a compact argument showing directly how to reconstruct a pointed map $\Bf:\BG\ptdto\BH$ from an abstract group homomorphism from $\abstr(G)$ to $\abstr(H)$, the second translates back and forth via our equivalence between abstract and concrete groups.



The statement we are after is


\begin{lemma}
  \label{lem:homomabstrconcr}
  If $G$ and $H$ are groups, then
$$\abstr:\Hom(G,H)\to\Hom^\abstr(\abstr(G),\abstr(H))$$
is an equivalence.
\end{lemma}
and the next two subsections offer two proofs.



\sususe{``Delooping'' a group homomorphism}
\label{sec:delooping} %after Coquand, after Deligne
We now explore the first approach.
It might be helpful to review \cref{lem:S1-delooping}
for a simple example of delooping in the special case of the circle.
Here we elaborate the general case.

\begin{proof}
  Suppose we are given an abstract group homomorphism
$$f:\Hom^\abstr(\abstr(G),\abstr(H))$$
and we explain how to build a map $g:\BG_\div \rightarrow \BH_\div$ with
a path $p:\shape_H = g(\shape_G)$ such that $p f(\omega) = g(\omega) p$
for all $\omega:\shape_G = \shape_G$ (so that $g$ is a ``delooping'' of $f$, that is, $f=\abstr(g)$).
\marginnote{We will thus have displayed a map $\mathrm{deloop}:\Hom^\abstr(\abstr(G),\abstr(H))\to\Hom(G,H)$ with $\abstr\,\mathrm{deloop}=\refl{}$. We leave it to the reader to prove that $\mathrm{deloop}\,\abstr=\refl{}$. }

To get an idea of our strategy, let us assume the problem solved. The map $g:\BG_\div\rightarrow \BH_\div$
will then send any path $\alpha:{\shape_G} = x$ to a path $g(\alpha):g({\shape_G}) = g(x)$
and so we get a family of paths $p(\alpha) \defequi g(\alpha) p$ in ${\shape_H} = g(x)$ such that
$$p(\alpha\omega) = g(\alpha)g(\omega)p
  = g(\alpha)pf(\omega) = p(\alpha)f(\omega)$$
for all $\omega:{\shape_G} = {\shape_G}$ and $\alpha : {\shape_G} = x$.

This suggests to introduce the following family
$$
C(x)~:=~ \sum_{y:\BH_\div}\sum_{p:({\shape_G}=x)\rightarrow ({\shape_H} = y)}~~~\prod_{\omega:{\shape_G}={\shape_G}}\prod_{\alpha:{\shape_G}=x}~
 p(\alpha\omega) = p(\alpha)f(\omega)
$$
 An element of $C(x)$ has three components, the last component being
 a proposition since $\BH_\div$ is a groupoid.

 The type $C({\shape_G})$ has a simpler description. An element of $C({\shape_G})$ is
 a pair $y,p$ such that $p(\alpha\omega) = p(\alpha)f(\omega)$ for
 $\alpha$ and $\omega$ in ${\shape_G}={\shape_G}$.
 Since $f$ is an abstract group homomorphism, this condition
 can be simplified to $p(\omega) = p(1_{\shape_G})f(\omega)$, and the map $p$
 is completely determined by $p(1_{\shape_G})$.
 Thus $C({\shape_G})$ is equal to $\sum_{y:\BH_\div}{\shape_H} = y$ and is contractible.


 It follows that we have
 $$
 \prod_{x:\BG_\div}~ ({\shape_G} = x)\rightarrow\iscontr~ C(x)
 $$
and so, since $\iscontr~C(x)$ is a proposition
 $$
 \prod_{x:\BG_\div}~ \Trunc{a = x}\rightarrow\iscontr~ C(x)
 $$
 Since $\BG_\div$ is connected, we have
 $\prod_{x:\BG_\div}\iscontr~ C(x)$
 and so, in particular, we have an element of $\prod_{x:\BG_\div}C(x)$.

 We get in this way a map $g:\BG_\div\rightarrow \BH_\div$
 together with a map $p:(a=x)\rightarrow ({\shape_H} = g(x))$ such that
 $p (\alpha\omega) = p(\alpha) f(\omega)$
 for all $\alpha$ in ${\shape_G}=x$ and $\omega$ in ${\shape_G}={\shape_G}$.
We have, for $\alpha:{\shape_G}=x$
$$\prod_{x':\BG_\div}\prod_{\lambda:x=x'}~p(\lambda\alpha) = g(\lambda)p(\alpha)$$
since this holds for $\lambda = 1_x$.
In particular, $p(\omega) = g(\omega)p(1_{\shape_G})$.

We also have $p(\omega) = p(1_{\shape_G})f(\omega)$, hence
$p(1_{\shape_G})g(\alpha) =  f(\alpha)p(1_{\shape_G})$
for all $\alpha:\shape_G=\shape_G$ and we have found a delooping of $f$.

%Security copy if things go wrong. BID: delete by May 1
%   Let $(X,a)$ and $(Y,b)$ be two pointed connected $1$-types.
% We suppose given a abstract group homomorphism
% $$f:a = a\rightarrow b = b$$
% and we explain how to build a map $g:X \rightarrow Y$ with
% a path $p:b = g(a)$ such that $p f(\omega) = g(\omega) p$
% for all $\omega:a = a$. (So $g$ is a ``delooping'' of $f$.)

% \medskip

% Let us assume the problem solved. The map $g:X\rightarrow Y$
% will then send any path $\alpha:a = x$ to a path $g(\alpha):g(a) = g(x)$
% and so we get a family of paths $p(\alpha) = g(\alpha) p$ in $b = g(x)$ such that
% $$p(\alpha\omega) = g(\alpha)g(\omega)p
%   = g(\alpha)pf(\omega) = p(\alpha)f(\omega)$$
% for all $\omega:a = a$ and $\alpha : a = x$.

% \medskip

% This suggests to introduce the following family
% $$
% C(x)~:=~ \sum_{y:Y}\sum_{p:(a=x)\rightarrow (b = y)}~~~\prod_{\omega:a=a}\prod_{\alpha:a=x}~
%  p(\alpha\omega) = p(\alpha)f(\omega)
% $$

%  An element of $C(x)$ has three components, the last component being
%  a proof since $Y$ is a $1$-type.

%  The type $C(a)$ has a simpler description. An element of $C(a)$ is
%  a pair $y,p$ such that $p(\alpha\omega) = p(\alpha)f(\omega)$ for
%  $\alpha$ and $\omega$ in $a=a$. Since $f$ is a group morphism, this condition
%  can be simplified to $p(\omega) = p(1_a)f(\omega)$, and the map $p$
%  is completely determined by $p(1_a)$.
%  Thus $C(a)$ is equal to $\sum_{y:Y}b = y$ and is contractible.

%  \medskip

%  It follows that we have
%  $$
%  \prod_{x:X}~ a = x\rightarrow\iscontr~ C(x)
%  $$
% and so, since $\iscontr~C(x)$ is a proposition
%  $$
%  \prod_{x:X}~ \Trunc{a = x}\rightarrow\iscontr~ C(x)
%  $$
%  Since $X$ is connected, we have
%  $\prod_{x:X}\iscontr~ C(x)$
%  and so, in particular, we have an element of $\prod_{x:X}C(x)$.

%  We get in this way a map $g:X\rightarrow Y$
%  together with a map $p:(a=x)\rightarrow (b = g(x))$ such that
%  $p (\alpha\omega) = p(\alpha) f(\omega)$
%  for all $\alpha$ in $a=x$ and $\omega$ in $a=a$.
% We have, for $\alpha:a=x$
% $$\prod_{x':X}\prod_{\lambda:x=x'}~p(\lambda\alpha) = g(\lambda)p(\alpha)$$
% since this holds for $\lambda = 1_x$.
% In particular, $p(\omega) = g(\omega)p(1_a)$.

% We also have $p(\omega) = p(1_a)f(\omega)$, hence
% $p(1_a)g(\alpha) =  f(\alpha)p(1_a)$
% for all $\alpha:a=a$ and we have found a delooping of $f$.
\end{proof}


\sususe{The concrete vs. abstract homomorphisms via torsors.}
\label{sec:absconctorsor}

The second approach to \cref{lem:homomabstrconcr} is as follows:


\begin{proof}
  The equivalence of $\pathsp{}^G:\BG\we(\typetorsor_G,\princ G)$ of \cref{lem:BGbytorsor} gives an equivalence
$$\pathsp{}:\Hom(G,H)\we((\typetorsor_G,\princ G)\to_*(\typetorsor_H,\princ H))
$$
Consider the map
$$A:((\typetorsor_G,\princ G))\to_*(\typetorsor_H,\princ H)\to \Hom^\abstr(\abstr(G),\abstr(H))$$
given by letting $A(f,p)$ be the composite
$$\xymatrix{\USymG\ar@{=}[d]^{\pathsp{}^G}_\downarrow&&&
  \USymH\ar@{=}[d]^{\pathsp{}^H}_\downarrow\\
  (\princ G=\princ G)\ar[r]^-f&
  (f\princ G=f\princ G)\ar@{=}[rr]^-{q\mapsto p^{-1}qp}_\to&&
  (\princ H=\princ H)
}$$
(together with the proof that this is an abstract group homomorphism).  We
are done if we show that $A$ is an equivalence.
\marginnote{The reason to complicate $\abstr$ this way is that it gets easier to write out the inverse function.}

If $(\phi,!):\Hom^\abstr(\abstr(G),\abstr(H))$ and $X:\BG\to\Set$ is a $G$-torsor, recall the induced $H$-torsor $\phi_*X$ from \cref{rem:inducedGsetfromabstracthomomorphisms} and the identity $\eta_\phi:\phi_*\princ G=\princ H$.
Let
$$B: \Hom^\abstr(\abstr(G),\abstr(H))\to ((\typetorsor_G,\princ G)\to_*(\typetorsor_H,\princ H)$$
be given by $B(\phi,!)=(\phi_*X,\eta_\phi)$

We show that $A$ and $B$ are inverse equivalences.  Given an abstract group homomorphism $(\phi,!):\Hom^\abstr(\abstr(G),\abstr(H))$, then $AB(\phi,!)$ has as underlying set map
$$\xymatrix{\USymG\ar@{=}[d]^{\pathsp{}^G}_\downarrow&&&
  \USymH\ar@{=}[d]^{\pathsp{}^H}_\downarrow\\
  (\princ G=\princ G)\ar[r]^-{\phi_*}&
  (\phi_*\princ G=\phi_*\princ G)\ar@{=}[rr]^-{q\mapsto \eta_\phi^{-1}q\eta_\phi}_\to&&
  (\princ H=\princ H),
}$$
and if we start with a $g:\USymG$, then $\pathsp{}^G$ sends it to $\pathsp g^G\oldequiv\preinv (g)$.  Furthermore, $\phi_*\preinv (g)$ is $[\id,\preinv (g)]$ which is sent to $\preinv (\phi(g))$ in $\princ H=\princ H$ which corresponds to $\phi(g):\USymH$ under $\pathsp{}^H$.  In other words, $AB(\phi,!)=(\phi,!)$.  The composite $BA$ is similar.
\end{proof}

\section{Actions}
\label{sec:Gsetsabstrconcr}
\marginnote{Recall from \cref{def:abstrGtorsors} that the type of $\abstr(G)$-set is
  $$\Set_{\abstr(G)}^\abstr\defequi \sum_{\mathcal X:\Set}\Hom_\abstr({\abstr(G)},\abstr(\Sigma_{\mathcal X})).$$}

Given a group $G$ it should by now come as no surprise that the type of $G$-sets is equivalent to the type of $\abstr(G)$-sets.
According to \cref{lem:homomabstrconcr}
$$\abstr:\Hom(G,\Sigma_{\mathcal X})\to\Hom^\abstr(\abstr(G),\abstr(\Sigma_{\mathcal X}))$$
is an equivalence, where the group $\Sigma_{\mathcal X}$ (as a pointed connected groupoid) is the component of the groupoid $\Set$, pointed at $\mathcal X$.  The component information is moot since we're talking about pointed maps from $\BG$ and we see that $\Hom(G,\Sigma_{\mathcal X})$ is equivalent to $\sum_{F:\BG_\div\to\Set}(\mathcal X=F(\shape_G))$.  Finally,
$$\mathrm{pr}:\sum_{\mathcal X}\sum_{F:\BG_\div\to\Set}(\mathcal X=F(\shape_G))\we
(\BG_\div\to\Set),\quad \mathrm{pr}(\mathcal X,F,p)\defequi F
$$
is an equivalence (since $\sum_{\mathcal X}(\mathcal X=F(\shape_G))$ is contractible).
Backtracking these equivalences we see that we have established
\begin{lemma}
  \label{lem:actionsconcreteandabstract}
  Let $G$ be a group.  Then the map
  $$\ev_{\shape_G}:\GSet\to\Set^\abstr_{\abstr(G)},\qquad \ev_{\shape_G}(X)\defequi(X(\shape_G),a_X)
$$
is an equivalence, where the homomorphism $a_X:\Hom^\abstr(\abstr(G), \abstr(\Sigma_{X(\shape_G)}))$ is given by transport $X:\USymG\defequi(\shape_G=\shape_G)\to (X(\shape_G)=X(\shape_G))$.
\end{lemma}
If $X$ is a $G$-set, $g:\USymG$ and $x:X(\shape_G)$, we seek forgiveness for writing $g\cdot x:X(\shape_G)$ instead of $\cast(a_X(g))(x)$.\footnote{and I ask forgiveness for strongly disliking the use of ``$\cast$'' as a name for some tacitly understood map!}

\begin{example}
  \label{ex:abstrandconj}
  Let $H$ and $G$ be groups.  Recall that the set of homomorphisms from $H$ to $G$ is a $G$-set in a natural way:
$$\Hom(H,G):\BG\to\Set,\quad \Hom(H,G)(y)\defequi \sum_{F:\BH_\div\to \BG_\div}(y=F(\shape_H)).$$

What abstract $\abstr(G)$-set does this correspond to?
In particular, under the equivalence $\abstr:\Hom(H,G)\to\Hom^\abstr(\abstr(H),\abstr(G))$, what is the corresponding action of $\abstr(G)$ on the abstract homomorphisms?

The answer is that $g:\USymG$ acts on $\Hom^\abstr(\abstr(H),\abstr(G))$ by postcomposing with conjugation $\conj^g$ by $g$ as defined in \cref{ex:conjhomo}.

Let us spell this out in some detail:
If $(F,p):\Hom(H,G)(\shape_G)\defequi
 \sum_{F:\BH_\div\to \BG_\div}(\shape_G=F(\shape_H))$ and $g:\USymG$, then $g\cdot(F,p)\defequi(F,p\,g^{-1})$.  If we show that the action of $g$ sends $\abstr(F,p)$ to $\conj^g\circ\abstr(F,p)$ we are done.

Recall that $\abstr(F,p)$ consists of the composite
$$\xymatrix{\USymH\ar[r]^-{F^=}&(F(\shape_H)=F(\shape_G))\ar[rr]^-{t\mapsto p^{-1}t\,p}&&\USymG},$$
(\ie $\abstr(F,p)$ applied to $q:\USymH $ is  $p^{-1}F^=(q)\,p$)  together with the proof that this is an abstract group homomorphism.
We see that $\abstr(F,p\,g^{-1})$ is given by conjugation:
$q\mapsto(p\,g^{-1})^{-1}F^=(q)\,(p\,g^{-1})=g\,(p^{-1}F^=(q)\,p)\,g^{-1}$, or in other words $\conj^g\circ\abstr(F,p)$.
\end{example}
For reference we list the conclusion of this example as a lemma:
\begin{lemma}\label{lem:abstrandconj}
  If $H$ and $G$ are groups, then the equivalence of \cref{lem:actionsconcreteandabstract} sends the $G$-set $\Hom(H,G)$ to the $\abstr(G)$-set $\Hom^\abstr(\abstr(H),\abstr(G))$ with action given by postcomposing with conjugation by elements of $\abstr(G)$.
\end{lemma}

If $f:\Hom(G,G')$ is a homomorphism, then precomposition with $\Bf:\BG\to \BG'$ defines a map $$f^*:(G'\text{-}\Set)\to(G\text{-}\Set).$$
\marginnote{Recall that \cref{lem:eq-mono-cover} told us that $f$ is an epimorphism precisely when $\USymf$ is a surjection.}
We will have the occasion to use the following result which essentially says that if $f:\Hom(G,G')$ is an epimorphism, then $f^*$ embeds the type of $G'$-sets as some of the components of the type of $G$-sets.
\begin{lemma}
  \label{lem:epifullyfaithful}
  Let $G$ and $G'$ be groups and let $f:\Hom(G,G')$ be an epimorphism.
  Then the map $f^*:(G'\text{-}\Set)\to(G\text{-}\Set)$ (induced by precomposition with $\Bf:\BG\to \BG'$) is ``fully faithful'' in the sense that if $X,Y$ are $G'$-sets, then
$$f^*:(X=Y)\to(f^*X=f^*Y)
$$
is an equivalence.
\end{lemma}
\begin{proof}
  Evaluation at $\shape_G$  yields an injective map
$$\mathrm{ev}_{\shape_G}:(f^*X=f^*Y)\to(X(f(\shape_G)=Y(f(\shape_G)))$$ and the composite
$$\mathrm{ev}_{\shape_G}f^*=\mathrm{ev}_{f(\shape_G)}:(X=Y)\to(X(f(\shape_G)=Y(f(\shape_G)))$$
 is the likewise injective, so $f^*:(X=Y)\to(f^*X=f^*Y)$ is injective.

For surjectivity, let $F':f^*X=f^*Y$ and write, for typographical convenience, $a:X(f(\shape_G)=Y(f(\shape_G))$ for $\mathrm{ev}_{\shape_G}F'\defequi F'_{\shape_G}$.
By the equivalence between $G$-sets and $\abstr(G)$-sets, $F'$ is uniquely pinned down by $a$ and the requirement that for all $g'=f(g)$ with $g:\USymG$ the diagram
$$\xymatrix{X(f(\shape_G))\ar@{=}[r]^{X({g'})}\ar@{=}[d]_{a}&
  X(f(\shape_G))\ar@{=}[d]_{a}\\
  Y(f(\shape_G))\ar@{=}[r]^{Y({g'})}&Y(f(\shape_G))}
$$
commutes.  Likewise, (using transport along the identity $p_f:\shape_{G'}=f(\shape_G)$) an $F:X=Y$ in the preimage of $a$ is pinned down by the commutativity of the same diagram, but with $g':f(\shape_G)=f(\shape_G)$ arbitrary (an a priori more severe requirement, again reflecting injectivity).   However, when $f:\USymG\to\USymG'$ is surjective these requirements coincide, showing that $f^*$ is an equivalence.


% Fix for the moment an  $a:X(f(\shape_G)=Y(f(\shape_G))$

% Now, by transport along the identity $p_f:\shape_{G'}=f(\shape_G)$ and the equivalence between $G'$-sets and $\abstr(G')$-sets, an identity $F':X=Y$ of $G'$-sets is uniquely pinned down by an identity $F'_{f(\shape_G)}:X(f(\shape_G)=Y(f(\shape_G))$ together with the proposition that for all $g':f(\shape_G)=f(\shape_G)$ the diagram $$\xymatrix{X(f(\shape_G))\ar@{=}[r]^{X_{g'}}\ar@{=}[d]_{F'_{f(\shape_G)}}&
%   X(f(\shape_G))\ar@{=}[d]_{F'_{f(\shape_G)}}\\
%   Y(f(\shape_G))\ar@{=}[r]^{Y_{g'}}&Y(f(\shape_G))}
% $$
% commutes.  Likewise, an identity $F:f^*X=f^*Y$ is given by exactly the same data, except that the diagram is only required to commute for $g'=f(g)$ for all $g:\USymG$.  But when $f:\USymG\to\USymG'$ these requirements coincide.


% ; $F:X=Y$ is in the preimage of $a:X(f(\shape_G)=Y(f(\shape_G))$ if and only if $a=F_{f(\shape_G)}$ and for all $g':f(\shape_G)=f(\shape_G)$ the diagram
% $$\xymatrix{X(f(\shape_G))\ar@{=}[r]^{X_{g'}}\ar@{=}[d]_{F_{f(\shape_G)}}&
%   X(f(\shape_G))\ar@{=}[d]_{F_{f(\shape_G)}}\\
%   Y(f(\shape_G))\ar@{=}[r]^{Y_{g'}}&Y(f(\shape_G))}
% $$
% commutes.  However, since $f$ is surjective there is a $g:\USymG$ so that $g'=f(g)$.  Therefore, anything in $f^*X=f^*Y$ which is in the preimage of $a$ is in the image of $f^*:X=Y$ and we have shown that $f^*$ is also a surjection.
\end{proof}

%%% Local Variables:
%%% mode: LaTeX
%%% fill-column: 144
%%% latex-block-names: ("lemma" "theorem" "remark" "definition" "corollary" "fact" "properties" "conjecture" "proof" "question" "proposition" "exercise")
%%% TeX-master: "book"
%%% TeX-command-extra-options: "-fmt=macros"
%%% compile-command: "make book.pdf"
%%% End:
